Tree_calculus/Equal.v
@@ -25,18 +25,18 @@
 Require Import ArithRing Bool Max Omega.
 Require Import IntensionalLib.SF_calculus.Test.  
 Require Import IntensionalLib.SF_calculus.General.  
-Require Import IntensionalLib.Wave_as_SF.SF_Terms.  
-Require Import IntensionalLib.Wave_as_SF.SF_Tactics.  
-Require Import IntensionalLib.Wave_as_SF.SF_reduction.  
-Require Import IntensionalLib.Wave_as_SF.SF_Normal.  
-Require Import IntensionalLib.Wave_as_SF.SF_Closed.  
-Require Import IntensionalLib.Wave_as_SF.Substitution.  
-Require Import IntensionalLib.Wave_as_SF.SF_Eval.  
-Require Import IntensionalLib.Wave_as_SF.Star.  
-Require Import IntensionalLib.Wave_as_SF.Wait.  
-Require Import IntensionalLib.Wave_as_SF.Fixpoints.  
-Require Import IntensionalLib.Wave_as_SF.Wave_Factor.
-Require Import IntensionalLib.Wave_as_SF.Wave_Factor2.
+Require Import IntensionalLib.Tree_calculus.Tree_Terms.  
+Require Import IntensionalLib.Tree_calculus.Tree_Tactics.  
+Require Import IntensionalLib.Tree_calculus.Tree_reduction.  
+Require Import IntensionalLib.Tree_calculus.Tree_Normal.  
+Require Import IntensionalLib.Tree_calculus.Tree_Closed.  
+Require Import IntensionalLib.Tree_calculus.Substitution.  
+Require Import IntensionalLib.Tree_calculus.Tree_Eval.  
+Require Import IntensionalLib.Tree_calculus.Star.  
+Require Import IntensionalLib.Tree_calculus.Wait.  
+Require Import IntensionalLib.Tree_calculus.Fixpoints.  
+Require Import IntensionalLib.Tree_calculus.Wave_Factor.
+Require Import IntensionalLib.Tree_calculus.Wave_Factor2.
 
 
 Lemma subst_rec_closed_Fop: 
