Tree_calculus/Wave_Factor2.v
@@ -16,7 +16,7 @@
 (**********************************************************************)
 
 (**********************************************************************)
-(*                         Wave_Factor.v                              *)
+(*                        Wave_Factor2.v                              *)
 (*                                                                    *)
 (*                          Barry Jay                                 *)
 (*                                                                    *)
@@ -25,15 +25,15 @@
 Require Import Arith Omega List Max.
 Require Import IntensionalLib.SF_calculus.Test.  
 Require Import IntensionalLib.SF_calculus.General.  
-Require Import IntensionalLib.Wave_as_SF.SF_Terms.  
-Require Import IntensionalLib.Wave_as_SF.SF_Tactics.  
-Require Import IntensionalLib.Wave_as_SF.SF_reduction.  
-Require Import IntensionalLib.Wave_as_SF.SF_Normal.  
-Require Import IntensionalLib.Wave_as_SF.SF_Closed.  
-Require Import IntensionalLib.Wave_as_SF.Substitution.  
-Require Import IntensionalLib.Wave_as_SF.SF_Eval.  
-Require Import IntensionalLib.Wave_as_SF.Star.  
-Require Import IntensionalLib.Wave_as_SF.Wave_Factor.  
+Require Import IntensionalLib.Tree_calculus.Tree_Terms.  
+Require Import IntensionalLib.Tree_calculus.Tree_Tactics.  
+Require Import IntensionalLib.Tree_calculus.Tree_reduction.  
+Require Import IntensionalLib.Tree_calculus.Tree_Normal.  
+Require Import IntensionalLib.Tree_calculus.Tree_Closed.  
+Require Import IntensionalLib.Tree_calculus.Substitution.  
+Require Import IntensionalLib.Tree_calculus.Tree_Eval.  
+Require Import IntensionalLib.Tree_calculus.Star.  
+Require Import IntensionalLib.Tree_calculus.Wave_Factor.  
 
 
 
